rustfrontend/Clightgenproof.v
@@ -1185,47 +1185,6 @@ Proof.
     TrivialInject. eapply Val.inject_ptr; eauto. inv H2. 
   Qed. 
 
-Lemma extcall_free_injp: forall se tse v tv m m' tm t j Hm,
-    extcall_free_sem se [v] m t Vundef m' ->
-    Val.inject j v tv ->
-    exists tm' Hm',
-      extcall_free_sem tse [tv] tm t Vundef tm'
-      /\ injp_acc (injpw j m tm Hm) (injpw j m' tm' Hm').
-Proof.
-  intros until Hm.
-  intros FREE VINJ.
-  inv FREE. inv VINJ.
-  exploit Mem.load_inject; eauto.
-  intros (v2 & LOAD & VINJ).
-  exploit Mem.free_parallel_inject; eauto.
-  intros (m2' & TFREE & MINJ).
-  assert (P: Mem.range_perm m b (Ptrofs.unsigned lo - size_chunk Mptr) (Ptrofs.unsigned lo + Ptrofs.unsigned sz) Cur Freeable).
-    eapply Mem.free_range_perm; eauto.
-  (* refer the proof of extcall_free in Event: use address_inject *)  
-  exploit Mem.address_inject. eapply Hm.
-  apply Mem.perm_implies with Freeable; auto with mem.
-  apply P. instantiate (1 := lo).
-  generalize (size_chunk_pos Mptr); lia. eauto.
-  intros EQ.
-  assert (injp_acc (injpw j m tm Hm) (injpw j m' m2' MINJ)).
-  replace (Ptrofs.unsigned lo + Ptrofs.unsigned sz) with ((Ptrofs.unsigned lo - size_chunk Mptr) + (size_chunk Mptr + Ptrofs.unsigned sz)) in * by lia.
-  exploit injp_acc_free; eauto. 
-  assert (v2 = Vptrofs sz).
-  { unfold Vptrofs in *; destruct Archi.ptr64; inv VINJ; auto. }
-  subst.
-  exists m2', MINJ. split; auto.  
-  econstructor. erewrite <- LOAD. f_equal. lia.
-  auto. 
-  rewrite ! EQ. rewrite <- TFREE. f_equal; lia.
-  auto.
-  (* case 2 *)
-  exists tm, Hm. split.
-  replace tv with Vnullptr.
-  econstructor.
-  unfold Vnullptr in *.
-  destruct (Archi.ptr64); inv VINJ; auto.
-  reflexivity.
-Qed.  
   
 (* use injp_acc to prove inj_incr *)
 Lemma injp_acc_inj_incr: forall f f' m1 m2 m1' m2' Hm Hm',
